More field proofs

main.dfy
@@ -1,4 +1,4 @@
-type RR(0)
+type RR(00) // 00 = nonempty
 
 ghost const Zero: RR
 ghost const One: RR
@@ -63,22 +63,110 @@ lemma NegationOfNegation(x: RR)
 
 	assert neg(neg(x)) == x; // (1) + x == (2) + x
 }
-	
 
-lemma ZeroIsUnique(x: RR)
-	requires H: (forall y: RR :: add(y, x) == Zero)
-	ensures x == Zero
+lemma NegIsUnique(x: RR, y: RR)
+	requires add(x, y) == Zero
+	ensures y == neg(x)
 {
-	assert Zero == add(Zero, x) by {reveal H;}
-	assert add(Zero, x) == add(x, Zero) by {Conmutativity(x, Zero);}
-	assert add(x, Zero) == x by {Neutral(x);}
+	assert y == add(y, add(x, neg(x))) by {Neutral(y);}
+	assert add(y, add(x, neg(x))) == add(add(y, x), neg(x)) by {Associativity(y, x, neg(x));}
+	assert add(add(y, x), neg(x)) == add(add(x, y), neg(x)) by {Conmutativity(x, y);}
+	assert add(add(x, y), neg(x)) == add(Zero, neg(x));
+	assert add(Zero, neg(x)) == add(neg(x), Zero)           by {Conmutativity(Zero, neg(x));}
+	assert add(neg(x), Zero) == neg(x)                      by {Neutral(neg(x));}
 }
 
-lemma OneIsUnique(x: RR)
-	requires H: (forall y: RR :: mult(y, x) == One)
-	ensures x == One
+lemma InvIsUnique(x: RR, y: RR)
+	requires mult(x, y) == One
+	requires x != Zero
+	ensures y == inv(x)
 {
-	assert One == mult(One, x) by {reveal H;}
-	assert mult(One, x) == mult(x, One) by {Conmutativity(x, One);}
-	assert mult(x, One) == x by {Neutral(x);}
+	assert y == mult(y, mult(x, inv(x))) by {Neutral(y);}
+	assert mult(y, mult(x, inv(x))) == mult(mult(y, x), inv(x)) by {Associativity(y, x, inv(x));}
+	assert mult(mult(y, x), inv(x)) == mult(mult(x, y), inv(x)) by {Conmutativity(x, y);}
+	assert mult(mult(x, y), inv(x)) == mult(One, inv(x));
+	assert mult(One, inv(x)) == mult(inv(x), One)               by {Conmutativity(One, inv(x));}
+	assert mult(inv(x), One) == inv(x)                          by {Neutral(inv(x));}
+}
+
+lemma InversesAreUnique()
+	ensures forall x: RR, y: RR ::
+		((add(x, y) == Zero) ==> (y == neg(x)))
+		&& ((x != Zero && mult(x, y) == One) ==> (y == inv(x)))
+{
+	forall x: RR, y: RR
+		ensures ((add(x, y) == Zero) ==> (y == neg(x)))
+			&& ((x != Zero && mult(x, y) == One) ==> (y == inv(x)))
+	{
+		if add(x, y) == Zero {
+			assert y == neg(x) by {NegIsUnique(x, y);}
+		}
+		if x != Zero && mult(x, y) == One {
+			assert y == inv(x) by {InvIsUnique(x, y);}
+		}
+	}
+}
+
+lemma AnythingTimesZeroIsZero(x: RR)
+	ensures mult(x, Zero) == Zero
+{
+	assert mult(x, Zero) == add(mult(x, Zero), Zero)                                     by {Neutral(mult(x, Zero));}
+	assert mult(x, Zero) == add(mult(x, Zero), add(mult(x, Zero), neg(mult(x, Zero))));
+	assert mult(x, Zero) == add(add(mult(x, Zero), mult(x, Zero)), neg(mult(x, Zero)))   by {Associativity(mult(x, Zero), mult(x, Zero), neg(mult(x, Zero)));}
+	assert mult(x, Zero) == add(mult(x, add(Zero, Zero)), neg(mult(x, Zero)))            by {Distribuitivity(x, Zero, Zero);}
+	assert mult(x, Zero) == add(mult(x, Zero), neg(mult(x, Zero)))                       by {Neutral(Zero);}
+	assert mult(x, Zero) == Zero;
+}
+
+lemma InverseIsNeverZero(x: RR)
+	requires x != Zero
+	ensures inv(x) != Zero
+{
+	if inv(x) == Zero {
+		assert mult(x, inv(x)) == Zero by {AnythingTimesZeroIsZero(x);}
+		assert Zero != One             by {Neutral(Zero);}
+	}
+}
+
+lemma InverseOfInverse(x: RR)
+	requires x != Zero
+	ensures inv(x) != Zero
+	ensures inv(inv(x)) == x
+{
+	assert inv(x) != Zero by {InverseIsNeverZero(x);}
+
+	assert mult(inv(x), inv(inv(x))) == One; // (1)
+	assert mult(x, inv(x)) == One;           // (2)
+
+	// (2)
+	assert mult(One, x) == mult(x, mult(inv(x), x)) by {Associativity(x, inv(x), x);}
+	assert mult(One, x) == mult(x, mult(x, inv(x))) by {Conmutativity(inv(x), x);}
+	assert mult(One, x) == mult(x, One);
+	assert mult(One, x) == x                      by {Neutral(x);}
+
+	// (1)
+	assert mult(One, x) == mult(mult(inv(inv(x)), inv(x)), x) by {Conmutativity(inv(inv(x)), inv(x));}
+	assert mult(One, x) == mult(inv(inv(x)), mult(inv(x), x)) by {Associativity(inv(inv(x)), inv(x), x);}
+	assert mult(One, x) == mult(inv(inv(x)), mult(x, inv(x))) by {Conmutativity(inv(x), x);}
+	assert mult(One, x) == mult(inv(inv(x)), One);
+	assert mult(One, x) == inv(inv(x))                      by {Neutral(inv(inv(x)));}
+
+	assert inv(inv(x)) == x; // (1) * x == (2) * x
+}
+
+lemma ZeroIsUnique(x: RR, y: RR)
+	requires add(x, y) == x
+	ensures y == Zero
+{
+	assert add(add(x, y), neg(x)) == add(y, add(x, neg(x))) by {Conmutativity(x, y); Associativity(y, x, neg(x));}
+	assert add(add(x, y), neg(x)) == y                      by {Neutral(y);}
+}
+
+lemma OneIsUnique(x: RR, y: RR)
+	requires mult(x, y) == x
+	requires x != Zero
+	ensures y == One
+{
+	assert mult(mult(x, y), inv(x)) == mult(y, mult(x, inv(x))) by {Conmutativity(x, y); Associativity(y, x, inv(x));}
+	assert mult(mult(x, y), inv(x)) == y                        by {Neutral(y);}
 }
